specs/lemmas/Spec.Hash.Incremental.fsti
@@ -22,5 +22,9 @@ private val _sync_decl : Type0
 
 include Spec.Hash.Incremental.Definitions
 
-val hash_is_hash_incremental (a: hash_alg) (input: bytes { S.length input `less_than_max_input_length` a }):
-  Lemma (S.equal (hash a input) (hash_incremental a input))
+val hash_is_hash_incremental' (a: hash_alg) (input: bytes { S.length input `less_than_max_input_length` a })
+  (l: output_length a):
+  Lemma (S.equal (hash' a input l) (hash_incremental a input l))
+
+let hash_is_hash_incremental (a: const_alg) (input: bytes { S.length input `less_than_max_input_length` a }) =
+  hash_is_hash_incremental' a input ()
